Done all the theorems and lemmas. Managed to proof the main theorem

bft2.v
@@ -1,30 +1,30 @@
 Require Import Coq.Arith.Arith.
 Require Import Coq.Bool.Bool.
 Require Export Coq.Strings.String.
-Require Import Coq.Logic.FunctionalExtensionality.
+Require Import Coq.Classes.RelationClasses.
 Require Import Coq.Lists.List.
 Import ListNotations.
 Require Import Maps.
 Require Coq.omega.Omega.
+Require Import String.
+Require Import Maps.
+Open Scope string_scope.
 
 Definition ReplicaId := string.
 
-
 Inductive Replica : Set :=
-| FaultyReplica : Replica
-| NFReplica : Replica.
+| FaultyReplica : ReplicaId -> Replica
+| NFReplica : ReplicaId -> Replica.
 
 Definition IsNonFaulty (r:Replica) :  Prop :=
   match r with 
-    | FaultyReplica => False
-    | NFReplica => True
+    | FaultyReplica _ => False
+    | NFReplica _ => True
   end.
-
-Print list.
 
 Definition State := list (Replica * (list nat)).
 
-Definition ReplicaFun := nat -> State -> State.
+Definition ReplicaFun := total_map nat -> State -> State.
 
 Definition nfrValue := 0.
 Definition faultyValue := 100.
@@ -36,42 +36,85 @@ Fixpoint multicast (st:State) (v:nat) :=
   | (r, msgs)::t => (r, v::msgs)::(multicast t v)
   end.
 
-Definition NFReplicaFun (msg:nat) (st:State) :=
-       multicast st msg.
+Definition NFReplicaFun (id : ReplicaId) (msgs: total_map nat) (st:State) :=
+       multicast st (msgs id).
 
-
-Definition FaultyReplicaFun (msg:nat) (st:State) :=
+Definition FaultyReplicaFun (id : ReplicaId) (msgs: total_map nat) (st:State) :=
        multicast st faultyValue.
 
 Definition GetReplicaFun (r:Replica) : ReplicaFun :=
   match r with
-  | FaultyReplica => FaultyReplicaFun
-  | NFReplica => NFReplicaFun
+  | FaultyReplica id => FaultyReplicaFun id
+  | NFReplica id => NFReplicaFun id
   end.
 
 Definition System := list Replica.
 
-Fixpoint countNFR_system (sys:System) :=
+Fixpoint countNFR_state (st:State) :=
+match st with
+  | nil  => 0
+  | (NFReplica _, _)::t => S (countNFR_state t)
+  | _::t => countNFR_state t
+  end.
+
+Fixpoint count_state (st:State) :=
+match st with
+  | nil  => 0
+  | _::t => S (countNFR_state t)
+  end.
+
+
+Fixpoint count_system (sys:System) :=
 match sys with
-  | nil => 0 
-  | NFReplica::sys' => S (countNFR_system sys')
-  | FaultyReplica::sys' => countNFR_system sys'
-end.
+  | nil  => 0
+  | _::t => S (count_system t)
+  end.
 
 Definition F := 10.
-Definition CompleteSystem (sys:System) := length sys = 3*F+1 /\ countNFR_system sys = 2*F+1.
-Definition QuorumReq := 2*F+1.
+Definition CompleteState (st:State) := count_state st = 3*F+1 /\ countNFR_state st = 2*F+1.
+Definition CompleteSystem (sys:System) := count_system sys = 3*F+1.
+Definition QuorumRequirement := 2*F+1.
 
 Definition initState (sys:list Replica) : State := ( (map (fun r => (r, nil)) sys)).
-Definition prePrep (sys:list Replica) := ( (map (fun r => nfrValue) sys)).
-Compute prePrep [FaultyReplica; NFReplica].
 
-Fixpoint ReplicateRequest (sys : System) (msg: list nat) (st : State):=
-match sys, msg with
-  | nil, nil => st
-  | (r::sys'), (m::mt) => (GetReplicaFun r) m (ReplicateRequest sys' mt st)
-  | _, _ => nil
+Definition newPrePrep (msgs : total_map nat) (r: Replica) : total_map nat := 
+    match r with 
+    | NFReplica id => msgs & {id --> nfrValue}
+    | FaultyReplica id => msgs & {id --> nfrValue}
+    end.
+
+Definition prePrep (sys:list Replica) := 
+    ( (fold_left newPrePrep sys (t_empty nfrValue) )).
+Compute prePrep [(FaultyReplica "0"); (NFReplica "1")].
+
+Definition PrePrepGte (msgs : total_map nat) (sys : System) :=
+    msgs = prePrep sys \/ exists sys', msgs = prePrep(sys'++sys).
+
+Lemma PrePrepGte_Ind : forall (msgs : total_map nat) (sys : System) (r:Replica),
+    PrePrepGte msgs (r::sys) -> PrePrepGte msgs sys.
+Proof. intros. destruct H. 
+  - unfold PrePrepGte. right. exists [r]. apply H.
+  - unfold PrePrepGte. right. destruct H. exists (app x [r]). rewrite <- app_assoc. apply H.
+Qed.
+
+Definition StateGte st sys := st = initState sys \/ exists sys', st = initState (sys'++sys).
+
+Lemma StateGte_Ind : forall (st : State) (sys : System) (r:Replica),
+    StateGte st (r::sys) -> StateGte st sys.
+Proof. intros. destruct H. 
+  - unfold StateGte. right. exists [r]. apply H.
+  - unfold StateGte. right. destruct H. exists (app x [r]). rewrite <- app_assoc. apply H.
+Qed.
+
+Axiom PrimaryNonFaulty : forall (sys:System) (msgs : total_map nat),
+      PrePrepGte msgs sys -> forall (id : ReplicaId), msgs id = nfrValue.
+
+Fixpoint ReplicateRequest (sys : System) (msgs: total_map nat) (st : State):=
+match sys with
+  | nil => st
+  | (r::sys') => (GetReplicaFun r) msgs (ReplicateRequest sys' msgs st)
   end.
+
 
 Fixpoint countNFR_msgs msgs :=
 match msgs with
@@ -83,7 +126,7 @@ end.
 Fixpoint GatherCertificates (st:State) :=
 match st with
   | nil => nil
-  | (NFReplica, msgs)::t => (countNFR_msgs msgs)::(GatherCertificates t)
+  | (NFReplica id, msgs)::t => (countNFR_msgs msgs)::(GatherCertificates t)
   | _::t => GatherCertificates t
 end.
 
@@ -93,49 +136,63 @@ match certs with
 | h::t => (S h) :: (incCertificates t)
 end.
 
-Lemma FaultyR_GatherCerts : forall (st:State) (m:nat),
-        GatherCertificates (FaultyReplicaFun m st) = GatherCertificates st.
+Lemma FaultyR_GatherCerts : forall (st:State) (id:ReplicaId) (msgs : total_map nat),
+        GatherCertificates (FaultyReplicaFun id msgs st) = GatherCertificates st.
 Proof. intros.
   induction st.
     - reflexivity.
     - destruct a. destruct r; simpl; rewrite <- IHst; reflexivity.
 Qed.
 
-Lemma NFR_GatherCerts : forall (st:State),
-        GatherCertificates (NFReplicaFun nfrValue st) = incCertificates (GatherCertificates st).
+Lemma NFR_GatherCerts : forall (st:State) (id : ReplicaId) (msgs : total_map nat) (sys:System),
+            PrePrepGte msgs ((NFReplica id)::sys)
+            -> GatherCertificates (NFReplicaFun id msgs st) = incCertificates (GatherCertificates st).
 Proof. intros.
    induction st.
     - reflexivity.
     - destruct a. destruct r.
       + simpl. apply IHst.
-      + simpl. rewrite IHst. reflexivity.
+      + simpl. rewrite <- IHst. unfold NFReplicaFun. 
+         rewrite (PrimaryNonFaulty (NFReplica id :: sys) msgs). reflexivity. assumption.
 Qed.
 
+
 Inductive LedgerAgreement : (list nat) -> Prop :=
-| qcAgreement : forall (certs : list nat), 
-            Forall (fun x => ~ (lt x QuorumReq)) certs -> LedgerAgreement certs.
+| qcAgreement : forall (certs : list nat),
+          Forall (fun x => ~ (lt x QuorumRequirement)) certs 
+            -> LedgerAgreement certs.
+
+Axiom LedgerAgreementEmpty : forall msgs st,
+        LedgerAgreement (GatherCertificates (ReplicateRequest [] msgs st)).
 
 Lemma IncCertificates_MaintainsLedger : forall (certs : list nat),
-      LedgerAgreement certs ->
-        LedgerAgreement (incCertificates certs).
+      LedgerAgreement certs -> LedgerAgreement (incCertificates certs).
 Proof. intros. induction H. constructor. induction certs.
   - simpl. constructor.
   - simpl. inversion H. constructor.
-    + admit.
+    + unfold not. intros. rewrite <- H4 in H2. unfold not in H2. destruct H2.
+       auto.
     + apply IHcerts. apply H3.
-Admitted. 
+Qed. 
 
-Lemma StateValid : forall (sys:System) (st:State) (msgs:list nat),
-        CompleteSystem sys ->
-        st = (initState sys) /\ msgs = (prePrep sys) ->
-          LedgerAgreement (GatherCertificates (ReplicateRequest sys msgs st)).
+Lemma StateValid : forall (sys:System) (st:State) (msgs:total_map nat),
+      PrePrepGte msgs sys /\ StateGte st sys ->
+            LedgerAgreement (GatherCertificates (ReplicateRequest sys msgs st)).
 Proof.
   intros sys. induction sys.
-    + intros. induction H. inversion H1.
-    + intros. induction H0. destruct a.
-      - simpl. rewrite H1. simpl. rewrite FaultyR_GatherCerts. apply IHsys.
-        { admit. } { split. admit. admit. }
-      - simpl. rewrite H1. simpl. rewrite NFR_GatherCerts. 
+    + intros. apply LedgerAgreementEmpty.
+    + intros. destruct H. destruct a.
+      - simpl. rewrite FaultyR_GatherCerts. apply IHsys.
+      { split. 
+          - apply (PrePrepGte_Ind msgs sys (FaultyReplica r)). assumption.
+          - apply (StateGte_Ind st sys (FaultyReplica r)). assumption.
+      }
+      - simpl. 
+        rewrite (NFR_GatherCerts (ReplicateRequest sys msgs st) r msgs sys). 
         apply IncCertificates_MaintainsLedger. apply IHsys.
-        { admit. } { split. admit. admit. }
-Admitted.
+         { split. 
+            - apply (PrePrepGte_Ind msgs sys (NFReplica r)). assumption.
+            - apply (StateGte_Ind st sys (NFReplica r)). assumption.
+         }
+         { auto. }
+Qed.
